Foundation/Modal/Logic/WellKnown.lean
@@ -17,10 +17,10 @@ import Foundation.Modal.Kripke.Hilbert.KDB
 import Foundation.Modal.Kripke.Hilbert.KT
 import Foundation.Modal.Kripke.Hilbert.KTB
 import Foundation.Modal.Kripke.Hilbert.S4
-import Foundation.Modal.Kripke.Hilbert.S4Dot2
-import Foundation.Modal.Kripke.Hilbert.S4Dot3
-import Foundation.Modal.Kripke.Hilbert.GrzDot2
-import Foundation.Modal.Kripke.Hilbert.GrzDot3
+import Foundation.Modal.Kripke.Hilbert.S4Point2
+import Foundation.Modal.Kripke.Hilbert.S4Point3
+import Foundation.Modal.Kripke.Hilbert.GrzPoint2
+import Foundation.Modal.Kripke.Hilbert.GrzPoint3
 import Foundation.Modal.Kripke.Hilbert.S5
 import Foundation.Modal.Kripke.Hilbert.Triv
 import Foundation.Modal.Kripke.Hilbert.Ver
@@ -149,12 +149,12 @@ protected abbrev Grz : Logic := Hilbert.Grz.logic
 lemma Grz.eq_ReflexiveTransitiveAntiSymmetricFiniteKripkeFrameClass_Logic : Logic.Grz = Kripke.FrameClass.finite_strict_preorder.logic
   := eq_Hilbert_Logic_KripkeFrameClass_Logic
 
-protected abbrev GrzDot2 : Logic := Hilbert.GrzDot2.logic
-lemma GrzDot2.eq_ReflexiveTransitiveAntiSymmetricConfluentFiniteKripkeFrameClass_Logic : Logic.GrzDot2 = Kripke.ReflexiveTransitiveAntiSymmetricConfluentFiniteFrameClass.logic
+protected abbrev GrzPoint2 : Logic := Hilbert.GrzPoint2.logic
+lemma GrzPoint2.eq_ReflexiveTransitiveAntiSymmetricConfluentFiniteKripkeFrameClass_Logic : Logic.GrzPoint2 = Kripke.ReflexiveTransitiveAntiSymmetricConfluentFiniteFrameClass.logic
   := eq_Hilbert_Logic_KripkeFiniteFrameClass_Logic
 
-protected abbrev GrzDot3 : Logic := Hilbert.GrzDot3.logic
-lemma GrzDot3.eq_ReflexiveTransitiveAntiSymmetricConnectedFiniteKripkeFrameClass_Logic : Logic.GrzDot3 = Kripke.ReflexiveTransitiveAntiSymmetricConnectedFiniteFrameClass.logic
+protected abbrev GrzPoint3 : Logic := Hilbert.GrzPoint3.logic
+lemma GrzPoint3.eq_ReflexiveTransitiveAntiSymmetricConnectedFiniteKripkeFrameClass_Logic : Logic.GrzPoint3 = Kripke.ReflexiveTransitiveAntiSymmetricConnectedFiniteFrameClass.logic
   := eq_Hilbert_Logic_KripkeFiniteFrameClass_Logic
 
 protected abbrev Triv : Logic := Hilbert.Triv.logic
