Foundation/Modal/Kripke/Hilbert/GrzPoint3.lean
@@ -1,5 +1,5 @@
 import Foundation.Modal.Kripke.Hilbert.Grz.Completeness
-import Foundation.Modal.Kripke.Hilbert.S4Dot3
+import Foundation.Modal.Kripke.Hilbert.S4Point3
 
 namespace LO.Modal
 
@@ -13,14 +13,14 @@ namespace Kripke
 
 abbrev ReflexiveTransitiveAntiSymmetricConnectedFiniteFrameClass : FiniteFrameClass := { F | Reflexive F.Rel ∧ Transitive F.Rel ∧ AntiSymmetric F.Rel ∧ Connected F.Rel }
 
-instance : ReflexiveTransitiveAntiSymmetricConnectedFiniteFrameClass.DefinedBy {Axioms.K (atom 0) (atom 1), Axioms.Grz (atom 0), Axioms.Dot3 (atom 0) (atom 1)} := by
-  have h₁ := restrictFin_definability {Axioms.Dot3 (atom 0) (atom 1)} ({F | Connected F}) $ ConnectedFrameClass.DefinedByDot3
+instance : ReflexiveTransitiveAntiSymmetricConnectedFiniteFrameClass.DefinedBy {Axioms.K (atom 0) (atom 1), Axioms.Grz (atom 0), Axioms.Point3 (atom 0) (atom 1)} := by
+  have h₁ := restrictFin_definability {Axioms.Point3 (atom 0) (atom 1)} ({F | Connected F}) $ ConnectedFrameClass.DefinedByPoint3
   have := @FiniteFrameClass.definedBy_inter
     ReflexiveTransitiveAntiSymmetricFiniteFrameClass
     ({Axioms.K (atom 0) (atom 1), Axioms.Grz (atom 0)})
     inferInstance
     { F | Connected F.Rel}
-    {Axioms.Dot3 (atom 0) (atom 1)}
+    {Axioms.Point3 (atom 0) (atom 1)}
     h₁;
   have e₁ :
     (ReflexiveTransitiveAntiSymmetricFiniteFrameClass ∩ {F | Connected F.Rel}) =
@@ -29,8 +29,8 @@ instance : ReflexiveTransitiveAntiSymmetricConnectedFiniteFrameClass.DefinedBy {
       simp;
       tauto;
   have e₂ :
-    ({Axioms.K (atom 0) (atom 1), Axioms.Grz (atom 0)} ∪ {Axioms.Dot3 (atom 0) (atom 1)}) =
-    ({Axioms.K (atom 0) (atom 1), Axioms.Grz (atom 0), Axioms.Dot3 (atom 0) (atom 1)} : Set (Formula ℕ)) := by
+    ({Axioms.K (atom 0) (atom 1), Axioms.Grz (atom 0)} ∪ {Axioms.Point3 (atom 0) (atom 1)}) =
+    ({Axioms.K (atom 0) (atom 1), Axioms.Grz (atom 0), Axioms.Point3 (atom 0) (atom 1)} : Set (Formula ℕ)) := by
       ext φ;
       constructor;
       . rintro (⟨_, _⟩ | _) <;> tauto;
@@ -44,16 +44,16 @@ instance : ReflexiveTransitiveAntiSymmetricConnectedFiniteFrameClass.IsNonempty 
 end Kripke
 
 
-namespace Hilbert.GrzDot3
+namespace Hilbert.GrzPoint3
 
 open Kripke.Grz
 
-instance Kripke.sound : Sound (Hilbert.GrzDot3) (Kripke.ReflexiveTransitiveAntiSymmetricConnectedFiniteFrameClass) := inferInstance
+instance Kripke.sound : Sound (Hilbert.GrzPoint3) (Kripke.ReflexiveTransitiveAntiSymmetricConnectedFiniteFrameClass) := inferInstance
 
-instance Kripke.consistent : Entailment.Consistent (Hilbert.GrzDot3) :=
+instance Kripke.consistent : Entailment.Consistent (Hilbert.GrzPoint3) :=
   Kripke.Hilbert.consistent_of_FiniteFrameClass ReflexiveTransitiveAntiSymmetricConnectedFiniteFrameClass
 
-instance complete : Complete (Hilbert.GrzDot3) (Kripke.ReflexiveTransitiveAntiSymmetricConnectedFiniteFrameClass) :=
+instance complete : Complete (Hilbert.GrzPoint3) (Kripke.ReflexiveTransitiveAntiSymmetricConnectedFiniteFrameClass) :=
   complete_of_mem_miniCanonicalFrame Kripke.ReflexiveTransitiveAntiSymmetricConnectedFiniteFrameClass $ by
     intro φ;
     refine ⟨miniCanonicalFrame.reflexive, miniCanonicalFrame.transitive, miniCanonicalFrame.antisymm, ?_⟩;
@@ -83,6 +83,6 @@ instance complete : Complete (Hilbert.GrzDot3) (Kripke.ReflexiveTransitiveAntiSy
       . sorry;
       . sorry;
 
-end Hilbert.GrzDot3
+end Hilbert.GrzPoint3
 
 end LO.Modal
